Tap

DeBruijnSSA/BinSyntax/Rewrite/Definitions.lean
@@ -41,8 +41,8 @@ inductive WfD.CongD (P : Ctx α ε → LCtx α → Region φ → Region φ → S
     β.WfD Γ (R ++ L) →
     (hG : ∀i : Fin n, (G i).WfD (⟨R.get (i.cast hR.symm), ⊥⟩::Γ) (R ++ L)) →
     (i : Fin n) →
-    CongD P (⟨R.get (i.cast hR.symm), ⊥⟩::Γ) (R ++ L) r r' →
-    CongD P Γ L (Region.cfg β n (Function.update G i r)) (Region.cfg β n (Function.update G i r'))
+    CongD P (⟨R.get (i.cast hR.symm), ⊥⟩::Γ) (R ++ L) (G i) g' →
+    CongD P Γ L (Region.cfg β n G) (Region.cfg β n (Function.update G i g'))
 
 def WfD.CongD.left {P : Ctx α ε → LCtx α → Region φ → Region φ → Sort _} {Γ L r r'}
   (toLeft : ∀{Γ L r r'}, P Γ L r r' → r.WfD Γ L) : CongD P Γ L r r' → r.WfD Γ L
@@ -55,10 +55,8 @@ def WfD.CongD.left {P : Ctx α ε → LCtx α → Region φ → Region φ → So
   | cfg_block R hR dβ dG i pr => WfD.cfg _ R hR dβ (λk => by
     if h : k = i then
       cases h
-      simp only [Function.update_same]
       exact (pr.left toLeft)
     else
-      simp only [ne_eq, h, not_false_eq_true, Function.update_noteq]
       exact dG k
   )
 
@@ -194,10 +192,10 @@ def TStepD.symm {Γ L} {r r' : Region φ} : TStepD Γ L r r' → TStepD Γ L r' 
   | terminal e e' d => terminal e' e d
 
 inductive TStep : (Γ : Ctx α ε) → (L : LCtx α) → (r r' : Region φ) → Prop
-  | step {Γ L r r'} : r.WfD Γ L → r'.WfD Γ L → StepD Γ.effect r r' → TStep Γ L r r'
-  | step_op {Γ L r r'} : r.WfD Γ L → r'.WfD Γ L → StepD Γ.effect r' r → TStep Γ L r r'
-  | initial {Γ L} : Γ.IsInitial → r.WfD Γ L → r'.WfD Γ L → TStep Γ L r r'
-  | terminal {Γ L} : e.WfD Γ ⟨Ty.unit, ⊥⟩ → e'.WfD Γ ⟨Ty.unit, ⊥⟩ → r.WfD (⟨Ty.unit, ⊥⟩::Γ) L
+  | step {Γ L r r'} : r.Wf Γ L → r'.Wf Γ L → StepD Γ.effect r r' → TStep Γ L r r'
+  | step_op {Γ L r r'} : r.Wf Γ L → r'.Wf Γ L → StepD Γ.effect r' r → TStep Γ L r r'
+  | initial {Γ L} : Γ.IsInitial → r.Wf Γ L → r'.Wf Γ L → TStep Γ L r r'
+  | terminal {Γ L} : e.Wf Γ ⟨Ty.unit, ⊥⟩ → e'.Wf Γ ⟨Ty.unit, ⊥⟩ → r.Wf (⟨Ty.unit, ⊥⟩::Γ) L
     → TStep Γ L (let1 e r) (let1 e' r)
 
 theorem TStep.symm {Γ L} {r r' : Region φ} : TStep Γ L r r' → TStep Γ L r' r
@@ -206,36 +204,192 @@ theorem TStep.symm {Γ L} {r r' : Region φ} : TStep Γ L r r' → TStep Γ L r'
   | initial i d d' => initial i d' d
   | terminal e e' d => terminal e' e d
 
-inductive WfD.Cong (P : Ctx α ε → LCtx α → Region φ → Region φ → Prop)
+theorem TStep.left {Γ L} {r r' : Region φ} : TStep Γ L r r' → r.Wf Γ L
+  | TStep.step d _ _ => d
+  | TStep.step_op d _ _ => d
+  | TStep.initial _ d _ => d
+  | TStep.terminal de _ dr => dr.let1 de
+
+theorem TStep.right {Γ L} {r r' : Region φ} : TStep Γ L r r' → r'.Wf Γ L
+  | TStep.step _ d _ => d
+  | TStep.step_op _ d _ => d
+  | TStep.initial _ _ d => d
+  | TStep.terminal _ de dr => dr.let1 de
+
+inductive Wf.Cong (P : Ctx α ε → LCtx α → Region φ → Region φ → Prop)
   : Ctx α ε → LCtx α → Region φ → Region φ → Prop
   | step : P Γ L r r' → Cong P Γ L r r'
-  | case_left : e.WfD Γ ⟨Ty.coprod A B, ⊥⟩ → Cong P (⟨A, ⊥⟩::Γ) L r r' → s.WfD (⟨B, ⊥⟩::Γ) L
+  | case_left : e.Wf Γ ⟨Ty.coprod A B, ⊥⟩ → Cong P (⟨A, ⊥⟩::Γ) L r r' → s.Wf (⟨B, ⊥⟩::Γ) L
     → Cong P Γ L (Region.case e r s) (Region.case e r' s)
-  | case_right : e.WfD Γ ⟨Ty.coprod A B, ⊥⟩ → r.WfD (⟨A, ⊥⟩::Γ) L → Cong P (⟨B, ⊥⟩::Γ) L s s'
+  | case_right : e.Wf Γ ⟨Ty.coprod A B, ⊥⟩ → r.Wf (⟨A, ⊥⟩::Γ) L → Cong P (⟨B, ⊥⟩::Γ) L s s'
     → Cong P Γ L (Region.case e r s) (Region.case e r s')
-  | let1 : e.WfD Γ ⟨A, e'⟩ → Cong P (⟨A, ⊥⟩::Γ) L r r'
-    → Cong P Γ L (Region.let1 e r) (Region.let1 e r')
-  | let2 : e.WfD Γ ⟨Ty.prod A B, e'⟩ → Cong P (⟨B, ⊥⟩::⟨A, ⊥⟩::Γ) L r r'
-    → Cong P Γ L (Region.let2 e r) (Region.let2 e r')
+  | let1 : a.Wf Γ ⟨A, e⟩ → Cong P (⟨A, ⊥⟩::Γ) L r r'
+    → Cong P Γ L (Region.let1 a r) (Region.let1 a r')
+  | let2 : a.Wf Γ ⟨Ty.prod A B, e⟩ → Cong P (⟨B, ⊥⟩::⟨A, ⊥⟩::Γ) L r r'
+    → Cong P Γ L (Region.let2 a r) (Region.let2 a r')
   | cfg_entry (R : LCtx α) :
     (hR : R.length = n) →
     Cong P Γ (R ++ L) β β' →
-    (∀i : Fin n, (G i).WfD (⟨R.get (i.cast hR.symm), ⊥⟩::Γ) (R ++ L)) →
+    (∀i : Fin n, (G i).Wf (⟨R.get (i.cast hR.symm), ⊥⟩::Γ) (R ++ L)) →
     Cong P Γ L (Region.cfg β n G) (Region.cfg β' n G)
   | cfg_block (R : LCtx α) :
     (hR : R.length = n) →
-    β.WfD Γ (R ++ L) →
-    (hG : ∀i : Fin n, (G i).WfD (⟨R.get (i.cast hR.symm), ⊥⟩::Γ) (R ++ L)) →
+    β.Wf Γ (R ++ L) →
+    (hG : ∀i : Fin n, (G i).Wf (⟨R.get (i.cast hR.symm), ⊥⟩::Γ) (R ++ L)) →
     (i : Fin n) →
-    Cong P (⟨R.get (i.cast hR.symm), ⊥⟩::Γ) (R ++ L) r r' →
-    Cong P Γ L (Region.cfg β n (Function.update G i r)) (Region.cfg β n (Function.update G i r'))
+    Cong P (⟨R.get (i.cast hR.symm), ⊥⟩::Γ) (R ++ L) (G i) g' →
+    Cong P Γ L (Region.cfg β n G) (Region.cfg β n (Function.update G i g'))
 
-def Eqv (φ)
-  [EffInstSet φ (Ty α) ε] [PartialOrder α] [SemilatticeSup ε] [OrderBot ε]
-  (Γ : Ctx α ε) (L : LCtx α)
-  := Quot (WfD.Cong (TStep (φ := φ)) Γ L)
+theorem Wf.Cong.left {P : Ctx α ε → LCtx α → Region φ → Region φ → Prop} {Γ L r r'}
+  (toLeft : ∀{Γ L r r'}, P Γ L r r' → r.Wf Γ L) : Wf.Cong P Γ L r r' → r.Wf Γ L
+  | Wf.Cong.step p => toLeft p
+  | Wf.Cong.case_left de pr ds => case de (pr.left toLeft) ds
+  | Wf.Cong.case_right de dr ps => case de dr (ps.left toLeft)
+  | Wf.Cong.let1 de pr => Wf.let1 de (pr.left toLeft)
+  | Wf.Cong.let2 de pr => Wf.let2 de (pr.left toLeft)
+  | Wf.Cong.cfg_entry R hR pβ dG => Wf.cfg _ R hR (pβ.left toLeft) dG
+  | Wf.Cong.cfg_block R hR dβ dG i pr => Wf.cfg _ R hR dβ (λk => by
+    if h : k = i then
+      cases h
+      exact (pr.left toLeft)
+    else
+      exact dG k
+  )
 
--- TODO: Eqv.br, Eqv.case, Eqv.let1, Eqv2.let2, Eqv.cfg ...
+theorem Wf.Cong.right {P : Ctx α ε → LCtx α → Region φ → Region φ → Prop} {Γ L r r'}
+  (toRight : ∀{Γ L r r'}, P Γ L r r' → r'.Wf Γ L) : Wf.Cong P Γ L r r' → r'.Wf Γ L
+  | Wf.Cong.step p => toRight p
+  | Wf.Cong.case_left de pr ds => case de (pr.right toRight) ds
+  | Wf.Cong.case_right de dr ps => case de dr (ps.right toRight)
+  | Wf.Cong.let1 de pr => Wf.let1 de (pr.right toRight)
+  | Wf.Cong.let2 de pr => Wf.let2 de (pr.right toRight)
+  | Wf.Cong.cfg_entry R hR pβ dG => Wf.cfg _ R hR (pβ.right toRight) dG
+  | Wf.Cong.cfg_block R hR dβ dG i pr => Wf.cfg _ R hR dβ (λk => by
+    if h : k = i then
+      cases h
+      simp only [Function.update_same]
+      exact (pr.right toRight)
+    else
+      simp only [ne_eq, h, not_false_eq_true, Function.update_noteq]
+      exact dG k
+  )
+
+theorem Wf.Cong.eqv_iff {P : Ctx α ε → LCtx α → Region φ → Region φ → Prop} {Γ L r r'}
+  (toLeft : ∀{Γ L r r'}, P Γ L r r' → r.Wf Γ L)
+  (toRight : ∀{Γ L r r'}, P Γ L r r' → r'.Wf Γ L)
+  (p : EqvGen (Wf.Cong P Γ L) r r') : r.Wf Γ L ↔ r'.Wf Γ L
+  := by induction p with
+  | rel _ _ h => exact ⟨λ_ => h.right toRight, λ_ => h.left toLeft⟩
+  | refl => rfl
+  | symm _ _ _ I => exact I.symm
+  | trans _ _ _ _ _ Il Ir => exact Il.trans Ir
+
+theorem Wf.Cong.case_left_eqv
+  {P : Ctx α ε → LCtx α → Region φ → Region φ → Prop}
+  (e : Term φ) (he : e.Wf Γ ⟨Ty.coprod A B, ⊥⟩)
+  (p : EqvGen (Wf.Cong P (⟨A, ⊥⟩::Γ) L) r r')
+  (s : Region φ) (hs : s.Wf (⟨B, ⊥⟩::Γ) L)
+  : EqvGen (Wf.Cong P Γ L) (Region.case e r s) (Region.case e r' s)
+  := by induction p with
+  | rel _ _ h => exact EqvGen.rel _ _ (h.case_left he hs)
+  | refl _ => exact EqvGen.refl _
+  | symm _ _ _ I => exact I.symm
+  | trans _ _ _ _ _ Il Ir => exact Il.trans _ _ _ Ir
+
+theorem Wf.Cong.case_right_eqv
+  {P : Ctx α ε → LCtx α → Region φ → Region φ → Prop}
+  (e : Term φ) (he : e.Wf Γ ⟨Ty.coprod A B, ⊥⟩)
+  (r : Region φ) (hr : r.Wf (⟨A, ⊥⟩::Γ) L)
+  (p : EqvGen (Wf.Cong P (⟨B, ⊥⟩::Γ) L) s s')
+  : EqvGen (Wf.Cong P Γ L) (Region.case e r s) (Region.case e r s')
+  := by induction p with
+  | rel _ _ h => exact EqvGen.rel _ _ (h.case_right he hr)
+  | refl _ => exact EqvGen.refl _
+  | symm _ _ _ I => exact I.symm
+  | trans _ _ _ _ _ Il Ir => exact Il.trans _ _ _ Ir
+
+theorem Wf.Cong.let1_eqv
+  {P : Ctx α ε → LCtx α → Region φ → Region φ → Prop}
+  (a : Term φ) (ha : a.Wf Γ ⟨A, e⟩)
+  (p : EqvGen (Wf.Cong P (⟨A, ⊥⟩::Γ) L) r r')
+  : EqvGen (Wf.Cong P Γ L) (Region.let1 a r) (Region.let1 a r')
+  := by induction p with
+  | rel _ _ h => exact EqvGen.rel _ _ (h.let1 ha)
+  | refl _ => exact EqvGen.refl _
+  | symm _ _ _ I => exact I.symm
+  | trans _ _ _ _ _ Il Ir => exact Il.trans _ _ _ Ir
+
+theorem Wf.Cong.let2_eqv
+  {P : Ctx α ε → LCtx α → Region φ → Region φ → Prop}
+  (a : Term φ) (ha : a.Wf Γ ⟨Ty.prod A B, e⟩)
+  (p : EqvGen (Wf.Cong P (⟨B, ⊥⟩::⟨A, ⊥⟩::Γ) L) r r')
+  : EqvGen (Wf.Cong P Γ L) (Region.let2 a r) (Region.let2 a r')
+  := by induction p with
+  | rel _ _ h => exact EqvGen.rel _ _ (h.let2 ha)
+  | refl _ => exact EqvGen.refl _
+  | symm _ _ _ I => exact I.symm
+  | trans _ _ _ _ _ Il Ir => exact Il.trans _ _ _ Ir
+
+theorem Wf.Cong.cfg_entry_eqv
+  {P : Ctx α ε → LCtx α → Region φ → Region φ → Prop}
+  (R : LCtx α) (hR : R.length = n)
+  (p : EqvGen (Wf.Cong P Γ (R ++ L)) β β')
+  (dG : ∀i : Fin n, (G i).Wf (⟨R.get (i.cast hR.symm), ⊥⟩::Γ) (R ++ L))
+  : EqvGen (Wf.Cong P Γ L) (Region.cfg β n G) (Region.cfg β' n G)
+  := by induction p with
+  | rel _ _ h => exact EqvGen.rel _ _ (h.cfg_entry R hR dG)
+  | refl _ => exact EqvGen.refl _
+  | symm _ _ _ I => exact I.symm
+  | trans _ _ _ _ _ Il Ir => exact Il.trans _ _ _ Ir
+
+theorem Wf.Cong.cfg_block_eqv
+  {P : Ctx α ε → LCtx α → Region φ → Region φ → Prop}
+  (R : LCtx α) (hR : R.length = n)
+  (β)
+  (dβ : β.Wf Γ (R ++ L))
+  (dG : ∀i : Fin n, (G i).Wf (⟨R.get (i.cast hR.symm), ⊥⟩::Γ) (R ++ L))
+  (i : Fin n)
+  (p : EqvGen (Wf.Cong P (⟨R.get (i.cast hR.symm), ⊥⟩::Γ) (R ++ L)) (G i) g')
+  (toLeft : ∀{Γ L r r'}, P Γ L r r' → r.Wf Γ L)
+  : EqvGen (Wf.Cong P Γ L) (Region.cfg β n G) (Region.cfg β n (Function.update G i g'))
+  := by
+  generalize hg : G i = g
+  rw [hg] at p
+  induction p generalizing G with
+  | rel _ _ h => sorry--exact EqvGen.rel _ _ (h.cfg_block R hR dβ dG i)
+  | refl _ =>
+    rw [<-hg, Function.update_eq_self]
+    exact EqvGen.refl _
+  | symm x y hxy I =>
+    have I := @I (Function.update G i x)
+    rw [Function.update_idem, <-hg, Function.update_eq_self] at I
+    apply (I _ (by simp)).symm
+    intro k
+    if h : k = i then
+      cases h
+      rw [Function.update_same]
+      sorry
+    else
+      rw [Function.update_noteq h]
+      exact dG k
+  | trans _ _ _ _ _ Il Ir =>
+    sorry
+
+def CStep (Γ : Ctx α ε) (L : LCtx α) (r r' : Region φ) : Prop
+  := Wf.Cong TStep Γ L r r'
+
+def InS.CStep {Γ : Ctx α ε} {L : LCtx α} (r r' : InS φ Γ L) : Prop
+  := Region.CStep Γ L r.val r'.val
+
+instance InS.Setoid (φ) [EffInstSet φ (Ty α) ε] (Γ : Ctx α ε) (L : LCtx α) : Setoid (InS φ Γ L)
+  := EqvGen.Setoid InS.CStep
+
+theorem InS.let1_congr {Γ : Ctx α ε} {L : LCtx α}
+  {r r' : InS φ _ L} (a : Term φ) (da : a.Wf Γ ⟨A, e⟩)
+  (hr : r ≈ r') : InS.let1 a da r ≈ InS.let1 a da r'
+  := sorry
+
+def Eqv (φ) [EffInstSet φ (Ty α) ε] (Γ : Ctx α ε) (L : LCtx α) := Quotient (InS.Setoid φ Γ L)
 
 end Region
 
